backends/lean/Aeneas/Std/Scalar/CoreConvertNum.lean
@@ -592,31 +592,31 @@ iscalar_no_isize def core.num.«%S».to_be_bytes (x : «%S») : Array I8 (%Size)
 # From Little-Endian
 -/
 uscalar_no_usize def core.num.«%S».from_le_bytes (a : Array U8 (%Size)#usize) : «%S» :=
-  ⟨ (BitVec.fromLEBytes (List.map U8.toBitVec a.toInt)).cast (by simp) ⟩
+  ⟨ (BitVec.fromLEBytes (List.map U8.toBitVec a.val)).cast (by simp) ⟩
 
 iscalar_no_isize def core.num.«%S».from_le_bytes (a : Array I8 (%Size)#usize) : «%S» :=
-  ⟨ (BitVec.fromLEBytes (List.map I8.toBitVec a.toInt)).cast (by simp) ⟩
+  ⟨ (BitVec.fromLEBytes (List.map I8.toBitVec a.val)).cast (by simp) ⟩
 
 /-!
 # From Big-Endian
 -/
 uscalar_no_usize def core.num.«%S».from_be_bytes (a : Array U8 (%Size)#usize) : «%S» :=
-  ⟨ (BitVec.fromBEBytes (List.map U8.toBitVec a.toInt)).cast (by simp) ⟩
+  ⟨ (BitVec.fromBEBytes (List.map U8.toBitVec a.val)).cast (by simp) ⟩
 
 iscalar_no_isize def core.num.«%S».from_be_bytes (a : Array I8 (%Size)#usize) : «%S» :=
-  ⟨ (BitVec.fromBEBytes (List.map I8.toBitVec a.toInt)).cast (by simp) ⟩
+  ⟨ (BitVec.fromBEBytes (List.map I8.toBitVec a.val)).cast (by simp) ⟩
 
 /-!
 # Progress theorems: To Little-Endian
 -/
 uscalar_no_usize @[step]
 theorem core.num.«%S».to_le_bytes.step_spec (x : «%S») :
-  lift (core.num.«%S».to_le_bytes x) ⦃ y => y.toInt = x.toBitVec.toLEBytes.map (@UScalar.mk UScalarTy.U8) ⦄ := by
+  lift (core.num.«%S».to_le_bytes x) ⦃ y => y.val = x.toBitVec.toLEBytes.map (@UScalar.mk UScalarTy.U8) ⦄ := by
   simp only [spec_ok, lift, to_le_bytes, UScalarTy.U8_numBits_eq]
 
 iscalar_no_isize @[step]
 theorem core.num.«%S».to_le_bytes.step_spec (x : «%S») :
-  lift (core.num.«%S».to_le_bytes x) ⦃ y => y.toInt = x.toBitVec.toLEBytes.map (@IScalar.mk IScalarTy.I8) ⦄ := by
+  lift (core.num.«%S».to_le_bytes x) ⦃ y => y.val = x.toBitVec.toLEBytes.map (@IScalar.mk IScalarTy.I8) ⦄ := by
   simp only [spec_ok, lift, to_le_bytes, IScalarTy.I8_numBits_eq]
 
 /-!
@@ -624,12 +624,12 @@ theorem core.num.«%S».to_le_bytes.step_spec (x : «%S») :
 -/
 uscalar_no_usize @[step]
 theorem core.num.«%S».from_le_bytes.step_spec (x : Array U8 (%Size)#usize) :
-  lift (core.num.«%S».from_le_bytes x) ⦃ y => y.toBitVec = (BitVec.fromLEBytes (x.toNat.map U8.toBitVec)).cast (by simp) ⦄ := by
+  lift (core.num.«%S».from_le_bytes x) ⦃ y => y.toBitVec = (BitVec.fromLEBytes (x.val.map U8.toBitVec)).cast (by simp) ⦄ := by
   simp only [spec_ok, lift, from_le_bytes]
 
 iscalar_no_isize @[step]
 theorem core.num.«%S».from_le_bytes.step_spec (x : Array I8 (%Size)#usize) :
-  lift (core.num.«%S».from_le_bytes x) ⦃ y => y.toBitVec = (BitVec.fromLEBytes (x.toInt.map I8.toBitVec)).cast (by simp) ⦄  := by
+  lift (core.num.«%S».from_le_bytes x) ⦃ y => y.toBitVec = (BitVec.fromLEBytes (x.val.map I8.toBitVec)).cast (by simp) ⦄  := by
   simp only [spec_ok, lift, from_le_bytes]
 
 end Std
