backends/lean/Aeneas/Std/Scalar/Rotate.lean
@@ -20,7 +20,7 @@ uscalar @[step_pure_def]
 def core.num.«%S».rotate_left : «%S» → U32 → «%S» := @UScalar.rotate_left .«%S»
 
 def IScalar.rotate_left {ty} (x : IScalar ty) (shift : U32) : IScalar ty :=
-  ⟨ x.toBitVec.rotateLeft shift.toInt ⟩
+  ⟨ x.toBitVec.rotateLeft shift.toNat ⟩
 
 /- [core::num::{u8}::rotate_left] -/
 iscalar @[step_pure_def]
@@ -37,7 +37,7 @@ uscalar @[step_pure_def]
 def core.num.«%S».rotate_right : «%S» → U32 → «%S» := @UScalar.rotate_right .«%S»
 
 def IScalar.rotate_right {ty} (x : IScalar ty) (shift : U32) : IScalar ty :=
-  ⟨ x.toBitVec.rotateLeft shift.toInt ⟩
+  ⟨ x.toBitVec.rotateLeft shift.toNat ⟩
 
 /- [core::num::{u8}::rotate_right] -/
 iscalar @[step_pure_def]
